src/dvspec/dafny/att_spec_proofs/fnc_inv.dfy
@@ -2035,101 +2035,92 @@ module Fnc_Inv
         assert process' == ret_check_for_next_queued_duty.state;        
     }  
 
-/*
-    lemma lemma_inv19_f_listen_for_attestation_shares(
-        process: DVCNodeState,
-        attestation_share: AttestationShare,
-        process': DVCNodeState
-    )
-    requires f_listen_for_attestation_shares.requires(process, attestation_share)
-    requires process' == f_listen_for_attestation_shares(process, attestation_share).state        
-    requires inv19_body(process)
-    ensures inv19_body(process')
-    {}
-
-    lemma lemma_inv19_f_resend_attestation_share(
-        process: DVCNodeState,
-        process': DVCNodeState)
-    requires f_resend_attestation_share.requires(process)
-    requires process' == f_resend_attestation_share(process).state        
-    requires inv19_body(process)
-    ensures inv19_body(process')
-    { } 
-
-    lemma lemma_inv19_add_block_to_bn(
+    lemma lemma_inv22_add_block_to_bn(
         s: DVCNodeState,
         block: BeaconBlock,
         s': DVCNodeState 
     )
     requires add_block_to_bn.requires(s, block)
     requires s' == add_block_to_bn(s, block)    
-    requires inv19_body(s)
-    ensures inv19_body(s')
+    requires inv22_body(s)
+    ensures inv22_body(s')
     { }
 
-    lemma lemma_inv19_f_start_next_duty(process: DVCNodeState, attestation_duty: AttestationDuty, process': DVCNodeState)
-    requires f_start_next_duty.requires(process, attestation_duty)
-    requires process' == f_start_next_duty(process, attestation_duty).state   
-    requires forall queued_duty: AttestationDuty | queued_duty in process.attestation_duties_queue ::
-                        attestation_duty.slot <= queued_duty.slot                              
-    requires inv19_body(process)
-    ensures inv19_body(process')
-    { } 
-
-    lemma lemma_inv19_f_listen_for_new_imported_blocks(
+    lemma lemma_inv22_f_listen_for_attestation_shares(
         process: DVCNodeState,
-        block: BeaconBlock,
+        attestation_share: AttestationShare,
         process': DVCNodeState
     )
-    requires f_listen_for_new_imported_blocks.requires(process, block)
-    requires process' == f_listen_for_new_imported_blocks(process, block).state        
-    requires inv19_body(process)
-    ensures inv19_body(process')
+    requires f_listen_for_attestation_shares.requires(process, attestation_share)
+    requires process' == f_listen_for_attestation_shares(process, attestation_share).state        
+    requires inv22_body(process)
+    ensures inv22_body(process')
+    {}
+
+    lemma lemma_inv22_f_start_next_duty(process: DVCNodeState, attestation_duty: AttestationDuty, process': DVCNodeState)
+    requires f_start_next_duty.requires(process, attestation_duty)
+    requires process' == f_start_next_duty(process, attestation_duty).state   
+    requires inv22_body(process)
+    ensures inv22_body(process')
+    { } 
+
+    lemma lemma_inv22_f_resend_attestation_share(
+        process: DVCNodeState,
+        process': DVCNodeState)
+    requires f_resend_attestation_share.requires(process)
+    requires process' == f_resend_attestation_share(process).state        
+    requires inv22_body(process)
+    ensures inv22_body(process')
+    { } 
+
+    lemma lemma_inv22_f_check_for_next_queued_duty(
+        process: DVCNodeState,
+        process': DVCNodeState
+    )
+    requires f_check_for_next_queued_duty.requires(process)
+    requires process' == f_check_for_next_queued_duty(process).state    
+    requires inv22_body(process)
+    ensures inv22_body(process')
+    decreases process.attestation_duties_queue
     {
-        var new_consensus_instances_already_decided := f_listen_for_new_imported_blocks_helper_1(process, block);
+        if  && process.attestation_duties_queue != [] 
+            && (
+                || process.attestation_duties_queue[0].slot in process.future_att_consensus_instances_already_decided
+                || !process.current_attestation_duty.isPresent()
+            )    
+        {            
+                if process.attestation_duties_queue[0].slot in process.future_att_consensus_instances_already_decided.Keys 
+                {
+                    var queue_head := process.attestation_duties_queue[0];
+                    var new_attestation_slashing_db := f_update_attestation_slashing_db(process.attestation_slashing_db, process.future_att_consensus_instances_already_decided[queue_head.slot]);
+                    var process_mod := process.(
+                        attestation_duties_queue := process.attestation_duties_queue[1..],
+                        future_att_consensus_instances_already_decided := process.future_att_consensus_instances_already_decided - {queue_head.slot},
+                        attestation_slashing_db := new_attestation_slashing_db,
+                        attestation_consensus_engine_state := updateConsensusInstanceValidityCheck(
+                            process.attestation_consensus_engine_state,
+                            new_attestation_slashing_db
+                        )                        
+                    );
+                    lemma_inv22_f_check_for_next_queued_duty(process_mod, process');
+                }
+                else
+                { 
+                    var process_mod := process.(
+                        attestation_duties_queue := process.attestation_duties_queue[1..]
+                    );     
+                    assert inv22_body(process_mod);
 
-        var att_consensus_instances_already_decided := process.future_att_consensus_instances_already_decided + new_consensus_instances_already_decided;
-
-        var future_att_consensus_instances_already_decided := 
-            f_listen_for_new_imported_blocks_helper_2(process, att_consensus_instances_already_decided);
-
-        var process :=
-                process.(
-                    future_att_consensus_instances_already_decided := future_att_consensus_instances_already_decided,
-                    attestation_consensus_engine_state := stopConsensusInstances(
-                                    process.attestation_consensus_engine_state,
-                                    att_consensus_instances_already_decided.Keys
-                    ),
-                    attestation_shares_to_broadcast := process.attestation_shares_to_broadcast - att_consensus_instances_already_decided.Keys,
-                    rcvd_attestation_shares := process.rcvd_attestation_shares - att_consensus_instances_already_decided.Keys                    
-                );    
-        
-        assert inv19_body(process);
-
-        if process.current_attestation_duty.isPresent() && process.current_attestation_duty.safe_get().slot in att_consensus_instances_already_decided
-        {
-            var decided_attestation_data := att_consensus_instances_already_decided[process.current_attestation_duty.safe_get().slot];
-            var new_attestation_slashing_db := f_update_attestation_slashing_db(process.attestation_slashing_db, decided_attestation_data);
-            var process := process.(
-                current_attestation_duty := None,
-                attestation_slashing_db := new_attestation_slashing_db,
-                attestation_consensus_engine_state := updateConsensusInstanceValidityCheck(
-                    process.attestation_consensus_engine_state,
-                    new_attestation_slashing_db
-                )                
-            );
-            
-            assert inv19_body(process);
-
-            lemma_inv19_f_check_for_next_queued_duty(process, process');
+                    lemma_inv22_f_start_next_duty(process_mod, process.attestation_duties_queue[0], process');
+                }
         }
         else
-        {               
-            assert inv19_body(process);
+        { 
+            assert process'.all_rcvd_duties == process.all_rcvd_duties;
         }
-    } 
+    }
 
-    lemma lemma_inv19_f_att_consensus_decided(
+    lemma lemma_inv22_f_att_consensus_decided(
         process: DVCNodeState,
         id: Slot,
         decided_attestation_data: AttestationData, 
@@ -2137,8 +2128,8 @@ module Fnc_Inv
     )
     requires f_att_consensus_decided.requires(process, id, decided_attestation_data)
     requires process' == f_att_consensus_decided(process, id, decided_attestation_data).state         
-    requires inv19_body(process)
-    ensures inv19_body(process')
+    requires inv22_body(process)
+    ensures inv22_body(process')
     {
         
         var local_current_attestation_duty := process.current_attestation_duty.safe_get();
@@ -2165,14 +2156,83 @@ module Fnc_Inv
             );
 
     
-        assert inv19_body(process);
+        assert inv22_body(process);
 
         var ret_check_for_next_queued_duty := f_check_for_next_queued_duty(process);
         
-        lemma_inv19_f_check_for_next_queued_duty(process, ret_check_for_next_queued_duty.state);
+        lemma_inv22_f_check_for_next_queued_duty(process, ret_check_for_next_queued_duty.state);
 
         assert process' == ret_check_for_next_queued_duty.state;        
     } 
-*/
+    
+    lemma lemma_inv22_f_listen_for_new_imported_blocks(
+        process: DVCNodeState,
+        block: BeaconBlock,
+        process': DVCNodeState
+    )
+    requires f_listen_for_new_imported_blocks.requires(process, block)
+    requires process' == f_listen_for_new_imported_blocks(process, block).state        
+    requires inv22_body(process)
+    ensures inv22_body(process')
+    {
+        var new_consensus_instances_already_decided := f_listen_for_new_imported_blocks_helper_1(process, block);
 
+        var att_consensus_instances_already_decided := process.future_att_consensus_instances_already_decided + new_consensus_instances_already_decided;
+
+        var future_att_consensus_instances_already_decided := 
+            f_listen_for_new_imported_blocks_helper_2(process, att_consensus_instances_already_decided);
+
+        var process :=
+                process.(
+                    future_att_consensus_instances_already_decided := future_att_consensus_instances_already_decided,
+                    attestation_consensus_engine_state := stopConsensusInstances(
+                                    process.attestation_consensus_engine_state,
+                                    att_consensus_instances_already_decided.Keys
+                    ),
+                    attestation_shares_to_broadcast := process.attestation_shares_to_broadcast - att_consensus_instances_already_decided.Keys,
+                    rcvd_attestation_shares := process.rcvd_attestation_shares - att_consensus_instances_already_decided.Keys                    
+                );    
+        
+        assert inv22_body(process);
+
+        if process.current_attestation_duty.isPresent() && process.current_attestation_duty.safe_get().slot in att_consensus_instances_already_decided
+        {
+            var decided_attestation_data := att_consensus_instances_already_decided[process.current_attestation_duty.safe_get().slot];
+            var new_attestation_slashing_db := f_update_attestation_slashing_db(process.attestation_slashing_db, decided_attestation_data);
+            var process := process.(
+                current_attestation_duty := None,
+                attestation_slashing_db := new_attestation_slashing_db,
+                attestation_consensus_engine_state := updateConsensusInstanceValidityCheck(
+                    process.attestation_consensus_engine_state,
+                    new_attestation_slashing_db
+                )                
+            );
+            
+            assert inv22_body(process);
+
+            lemma_inv22_f_check_for_next_queued_duty(process, process');
+        }
+        else
+        {               
+            assert inv22_body(process);
+        }
+    } 
+
+    lemma lemma_inv22_f_serve_attestation_duty(
+        process: DVCNodeState,
+        attestation_duty: AttestationDuty,
+        process': DVCNodeState
+    )  
+    requires f_serve_attestation_duty.requires(process, attestation_duty)
+    requires process' == f_serve_attestation_duty(process, attestation_duty).state
+    requires inv22_body(process)
+    ensures inv22_body(process')
+    {
+        var process_mod := process.(
+                attestation_duties_queue := process.attestation_duties_queue + [attestation_duty],
+                all_rcvd_duties := process.all_rcvd_duties + {attestation_duty}
+            );        
+        
+        lemma_inv22_f_check_for_next_queued_duty(process_mod, process');        
+    } 
 }
